stash

examples/ghc/lib/PatSyn.v
@@ -13,19 +13,23 @@ Require Coq.Program.Wf.
 (* Converted imports: *)
 
 Require BasicTypes.
+Require Data.Function.
 Require FieldLabel.
 Require GHC.Base.
 Require Name.
+Require TyCoRep.
 Require Unique.
 Require Var.
+Import GHC.Base.Notations.
 
 (* Converted type declarations: *)
 
 Inductive PatSyn : Type := MkPatSyn : Name.Name -> Unique.Unique -> list
-                                      unit -> BasicTypes.Arity -> bool -> list FieldLabel.FieldLabel -> list
-                                      Var.TyVar -> list unit -> unit -> list Var.TyVar -> list
-                                      unit -> unit -> unit -> (Var.Id * bool)%type -> option (Var.Id *
-                                                                                             bool)%type -> PatSyn.
+                                      TyCoRep.Type_ -> BasicTypes.Arity -> bool -> list FieldLabel.FieldLabel -> list
+                                      Var.TyVar -> list TyCoRep.TyBinder -> TyCoRep.ThetaType -> list
+                                      Var.TyVar -> list
+                                      TyCoRep.TyBinder -> TyCoRep.ThetaType -> TyCoRep.Type_ -> (Var.Id *
+                                      bool)%type -> option (Var.Id * bool)%type -> PatSyn.
 
 Definition psArgs (arg_0__ : PatSyn) :=
   match arg_0__ with
@@ -108,13 +112,62 @@ Admitted.
 
 (* Converted value declarations: *)
 
-Instance Eq___PatSyn : GHC.Base.Eq_ PatSyn := {}.
-Proof.
-Admitted.
+Local Definition Eq___PatSyn_op_zeze__ : PatSyn -> PatSyn -> bool :=
+  Data.Function.on _GHC.Base.==_ Unique.getUnique.
 
-Instance Ord__PatSyn : GHC.Base.Ord PatSyn := {}.
-Proof.
-Admitted.
+Local Definition Eq___PatSyn_op_zsze__ : PatSyn -> PatSyn -> bool :=
+  Data.Function.on _GHC.Base./=_ Unique.getUnique.
+
+Program Instance Eq___PatSyn : GHC.Base.Eq_ PatSyn := fun _ k =>
+    k {|GHC.Base.op_zeze____ := Eq___PatSyn_op_zeze__ ;
+      GHC.Base.op_zsze____ := Eq___PatSyn_op_zsze__ |}.
+
+Local Definition Ord__PatSyn_compare : PatSyn -> PatSyn -> comparison :=
+  Data.Function.on GHC.Base.compare Unique.getUnique.
+
+Local Definition Ord__PatSyn_op_zg__ : PatSyn -> PatSyn -> bool :=
+  Data.Function.on _GHC.Base.>_ Unique.getUnique.
+
+Local Definition Ord__PatSyn_op_zgze__ : PatSyn -> PatSyn -> bool :=
+  Data.Function.on _GHC.Base.>=_ Unique.getUnique.
+
+Local Definition Ord__PatSyn_op_zl__ : PatSyn -> PatSyn -> bool :=
+  Data.Function.on _GHC.Base.<_ Unique.getUnique.
+
+Local Definition Ord__PatSyn_op_zlze__ : PatSyn -> PatSyn -> bool :=
+  Data.Function.on _GHC.Base.<=_ Unique.getUnique.
+
+Local Definition Ord__PatSyn_min : PatSyn -> PatSyn -> PatSyn :=
+  fun x y => if Ord__PatSyn_op_zlze__ x y : bool then x else y.
+
+Local Definition Ord__PatSyn_max : PatSyn -> PatSyn -> PatSyn :=
+  fun x y => if Ord__PatSyn_op_zlze__ x y : bool then y else x.
+
+Program Instance Ord__PatSyn : GHC.Base.Ord PatSyn := fun _ k =>
+    k {|GHC.Base.op_zl____ := Ord__PatSyn_op_zl__ ;
+      GHC.Base.op_zlze____ := Ord__PatSyn_op_zlze__ ;
+      GHC.Base.op_zg____ := Ord__PatSyn_op_zg__ ;
+      GHC.Base.op_zgze____ := Ord__PatSyn_op_zgze__ ;
+      GHC.Base.compare__ := Ord__PatSyn_compare ;
+      GHC.Base.max__ := Ord__PatSyn_max ;
+      GHC.Base.min__ := Ord__PatSyn_min |}.
+
+(* Translating `instance Unique.Uniquable PatSyn.PatSyn' failed: OOPS! Cannot
+   find information for class Qualified "Unique" "Uniquable" unsupported *)
+
+(* Translating `instance Name.NamedThing PatSyn.PatSyn' failed: OOPS! Cannot
+   find information for class Qualified "Name" "NamedThing" unsupported *)
+
+(* Translating `instance Outputable.Outputable PatSyn.PatSyn' failed: OOPS!
+   Cannot find information for class Qualified "Outputable" "Outputable"
+   unsupported *)
+
+(* Translating `instance Outputable.OutputableBndr PatSyn.PatSyn' failed: OOPS!
+   Cannot find information for class Qualified "Outputable" "OutputableBndr"
+   unsupported *)
+
+(* Translating `instance Data.Data.Data PatSyn.PatSyn' failed: OOPS! Cannot find
+   information for class Qualified "Data.Data" "Data" unsupported *)
 
 Axiom mkPatSyn : forall {A : Type}, A.
 
@@ -151,6 +204,9 @@ Axiom patSynInstResTy : forall {A : Type}, A.
 Axiom pprPatSynType : forall {A : Type}, A.
 
 (* Unbound variables:
-     bool list op_zt__ option unit BasicTypes.Arity FieldLabel.FieldLabel
-     GHC.Base.Eq_ GHC.Base.Ord Name.Name Unique.Unique Var.Id Var.TyVar
+     bool comparison list op_zt__ option BasicTypes.Arity Data.Function.on
+     FieldLabel.FieldLabel GHC.Base.Eq_ GHC.Base.Ord GHC.Base.compare
+     GHC.Base.op_zeze__ GHC.Base.op_zg__ GHC.Base.op_zgze__ GHC.Base.op_zl__
+     GHC.Base.op_zlze__ GHC.Base.op_zsze__ Name.Name TyCoRep.ThetaType
+     TyCoRep.TyBinder TyCoRep.Type_ Unique.Unique Unique.getUnique Var.Id Var.TyVar
 *)
